SP1Operations/SubOperation.lean
@@ -6,7 +6,7 @@ namespace SubOperation
 
 /-- `SubOperation` should result in wrapping addition of the outputs.
 Note that we ignore `is_real` for now. -/
-def spec (cols : SubOperation (Fin p)) (a b : Word (Fin p)) : Prop :=
+def spec (cols : SubOperation BabyBear) (a b : Word BabyBear) : Prop :=
   a.isUInt32 → b.isUInt32 →
     a.toNat = (cols.toNat + b.toNat) % 2^32
 
@@ -14,8 +14,8 @@ def spec (cols : SubOperation (Fin p)) (a b : Word (Fin p)) : Prop :=
 Asserting expr 3: `(is_real * (is_real - 1))`
 Asserting expr 17: `(is_real * (((((((a[0] + 65536) - 1) - b[0]) - cols.value[0]) + 1) * 2013235201) * (((((((a[0] + 65536) - 1) - b[0]) - cols.value[0]) + 1) * 2013235201) - 1)))`
 Asserting expr 29: `(is_real * (((((((a[1] + 65536) - 1) - b[1]) - cols.value[1]) + ((((((a[0] + 65536) - 1) - b[0]) - cols.value[0]) + 1) * 2013235201)) * 2013235201) * (((((((a[1] + 65536) - 1) - b[1]) - cols.value[1]) + ((((((a[0] + 65536) - 1) - b[0]) - cols.value[0]) + 1) * 2013235201)) * 2013235201) - 1)))` -/
-def extractedConstraints (cols : SubOperation (Fin p))
-    (a b : Word (Fin p)) (is_real : Fin p) : Prop :=
+def extractedConstraints (cols : SubOperation BabyBear)
+    (a b : Word BabyBear) (is_real : BabyBear) : Prop :=
   is_real * (is_real - 1) = 0 ∧
   is_real * (((((((a[0] + 65536) - 1) - b[0]) - cols[0]) + 1) * 2013235201) *
     (((((((a[0] + 65536) - 1) - b[0]) - cols[0]) + 1) * 2013235201) - 1)) = 0 ∧
@@ -24,23 +24,23 @@ def extractedConstraints (cols : SubOperation (Fin p))
       (((((((a[1] + 65536) - 1) - b[1]) - cols[1]) + ((((((a[0] + 65536) - 1) - b[0]) - cols[0]) + 1) * 2013235201)) * 2013235201) - 1)) = 0
 
 /-- Cleaned up representation of the `SubOperation` constraints. -/
-def idealizedConstraints (cols : SubOperation (Fin p))
-    (a b : Word (Fin p)) : Prop :=
-  let carry0 : Fin p := 1
-  let carry1 : Fin p := (a[0] + base - 1 - b[0] - cols[0] + carry0) * baseInv
-  let carry2 : Fin p := (a[1] + base - 1 - b[1] - cols[1] + carry1) * baseInv
+def idealizedConstraints (cols : SubOperation BabyBear)
+    (a b : Word BabyBear) : Prop :=
+  let carry0 : BabyBear := 1
+  let carry1 : BabyBear := (a[0] + base - 1 - b[0] - cols[0] + carry0) * baseInv
+  let carry2 : BabyBear := (a[1] + base - 1 - b[1] - cols[1] + carry1) * baseInv
   carry1 * (carry1 - 1) = 0 ∧ -- isBool check
   carry2 * (carry2 - 1) = 0 -- isBool check
 
 /-- The idealized constraints are logically equivalent to the extracted ones when `is_real := 1` -/
 lemma extractedConstraints_iff_idealizedConstraints
-    (cols : SubOperation (Fin p)) (a b : Word (Fin p)) :
+    (cols : SubOperation BabyBear) (a b : Word BabyBear) :
     cols.extractedConstraints a b 1 ↔ cols.idealizedConstraints a b := by
   simp [extractedConstraints, idealizedConstraints, Word.isUInt32]
 
 /-- The extracted constraints on `SubOperation` imply the spec. -/
-theorem correct [Fact (Nat.Prime p)] (cols : SubOperation (Fin p))
-    (a b : Word (Fin p)) (hcols : cols.isUInt32) :
+theorem correct [Fact (Nat.Prime p)] (cols : SubOperation BabyBear)
+    (a b : Word BabyBear) (hcols : cols.isUInt32) :
     cols.idealizedConstraints a b → cols.spec a b := by
   -- Unfold the definitions of constraints and spec
   simp [idealizedConstraints, spec, sub_eq_zero, mul_eq_zero]
@@ -51,7 +51,7 @@ theorem correct [Fact (Nat.Prime p)] (cols : SubOperation (Fin p))
   all_goals -- In both cases can now reduce down to the `omega` linear constraint solver
   · rw [h1] at h2
     simp only [Fin.add_def, Fin.sub_def, Fin.ext_iff, p, Word.toNat, Word.isUInt32] at *
-    simp [] at *
+    simp [BabyBearPrime] at *
     omega
 
 end SubOperation
